examples/dm4free/FStar.DM4F.ExnSt.fst
@@ -25,42 +25,39 @@ let bind a b f g =
     | None -> None
     | Some (ret, s1) -> g ret s1
 
+let raise (a:Type) : exnst a = fun _ -> None
+
 (* Define the new effect using DM4F *)
 reifiable reflectable new_effect_for_free {
   EXNST: a:Type -> Effect with
     repr    = exnst;
     bind    = bind;
     return  = return
+  and effect_actions
+    raise   = raise
 }
 
-let pre  = EXNST.pre
-let post = EXNST.post
-let wp   = EXNST.wp
-let repr = EXNST.repr
-
 (* A lift from Pure *)
-inline let lift_pure_exnst (a:Type) (wp:pure_wp a) (h0:int) (p:post a) =
+inline let lift_pure_exnst (a:Type) (wp:pure_wp a) (h0:int) (p:EXNST.post a) =
         wp (fun a -> p (Some (a, h0)))
 sub_effect PURE ~> EXNST = lift_pure_exnst
 
 (* A lift "for free" from STINT to EXNST *)
 let lift (a: Type) (f: IntST.st a): exnst a =
-  fun h ->
-    let ret = f h in
-    Some ret
+  fun h -> let ret = f h in Some ret
 
 sub_effect IntST.STINT ~> EXNST {
   lift = lift
 }
 
 (* A lift from a previously defined state effect *)
-val lift_state_exnst_wp : (a:Type) -> IntST.wp a -> wp a
-let lift_state_exnst_wp a wp (h0:int) (p:post a) =
+val lift_state_exnst_wp : (a:Type) -> IntST.wp a -> EXNST.wp a
+let lift_state_exnst_wp a wp (h0:int) (p:EXNST.post a) =
         wp h0 (fun r -> p (Some r))
 
 val lift_state_exnst : (a:Type) ->
                        (wp:IntST.wp a) -> (f:IntST.repr a wp) ->
-                       repr a (lift_state_exnst_wp a wp)
+                       EXNST.repr a (lift_state_exnst_wp a wp)
 let lift_state_exnst a wp f =
         (* TODO: This fails without admit, but all seems correct *)
         fun h0 -> admit(); Some (f h0)
@@ -70,17 +67,10 @@ sub_effect IntST.STINT ~> EXNST {
   lift = lift_state_exnst
 }
 
-(* Action: raise an exception *)
-let action_raise (a:Type) : repr a (fun _ post -> post None) =
-  fun _ -> None
-
-reifiable let raise (a:Type) : EXNST a (fun _ post -> post None) =
-  EXNST.reflect (action_raise a)
-
 (* Pre-/postcondition variant *)
-effect ExnSt (a:Type) (req:pre) (ens:int -> option (a * int) -> GTot Type0) =
+effect ExnSt (a:Type) (req:EXNST.pre) (ens:int -> option (a * int) -> GTot Type0) =
        EXNST a
-         (fun (h0:int) (p:post a) -> req h0 /\ (forall r. (req h0 /\ ens h0 r) ==> p r))
+         (fun (h0:int) (p:EXNST.post a) -> req h0 /\ (forall r. (req h0 /\ ens h0 r) ==> p r))
 
 (* Total variant *)
 effect S (a:Type) =
@@ -101,13 +91,13 @@ let div_intrinsic i j =
     if j = 0 then (
         (* Despite the incr (implicitly lifted), the state is reset *)
         IntST.incr ();
-        raise int
+        EXNST.raise int
     ) else
         i / j
 
 reifiable let div_extrinsic (i:nat) (j:int) : S int =
     if j = 0 then
-        raise int
+        EXNST.raise int
     else
         i / j
 
